On note $1:=\mathbf{1}_{\Omega}$ la fonction constante égale à $1 \operatorname{sur} \Omega$ (souvent identifiée à 1 ).

On vérifie facilement que $\mathbf{1}_{A^{c}}=1-\mathbf{1}_{A}$ et $\mathbf{1}_{A \cap B}=\mathbf{1}_{A} \mathbf{1}_{B}$.

Comme $A \cup B=\left(A^{c} \cap B^{c}\right)^{c}$, les formules précédentes donnent :

$$
\mathbf{1}_{A \cup B}=\mathbf{1}-\left(\left(\mathbf{1}-\mathbf{1}_{A}\right)\left(\mathbf{1}-\mathbf{1}_{B}\right)\right)=\mathbf{1}_{A}+\mathbf{1}_{B}-\mathbf{1}_{A} \mathbf{1}_{B}
$$
