1. Case $n=2$ :

Since $\mathbf{P}\left(A_{1} \cup A_{2}\right) \geqslant \mathbf{P}\left(A_{1}\right)=1$, one can write:

$$
\mathbf{P}\left(A_{1} \cap A_{2}\right)=\mathbf{P}\left(A_{1}\right)+\mathbf{P}\left(A_{2}\right)-\mathbf{P}\left(A_{1} \cup A_{2}\right)=1+1-1=1
$$

Case $n=3:($ not necessary but allows one to get an idea on how it works) Note that:

$$
\mathbf{P}\left(A_{1} \cup A_{2} \cup A_{3}\right)=\mathbf{P}\left(\left(A_{1} \cup A_{2}\right) \cup A_{3}\right)=\mathbf{P}\left(A_{1} \cup A_{2}\right)+\mathbf{P}\left(A_{3}\right)-\mathbf{P}\left(\left(A_{1} \cup A_{2}\right) \cap A_{3}\right)
$$

Besides, since $\mathbf{P}\left(A_{1} \cup A_{2} \cup A_{3}\right) \geqslant \mathbf{P}\left(A_{1}\right)=1$, one can write:

$$
\begin{equation*}
I_{3}:=\mathbf{P}\left(\left(A_{1} \cup A_{2}\right) \cap A_{3}\right)=\mathbf{P}\left(A_{1} \cup A_{2}\right)+\mathbf{P}\left(A_{3}\right)-\mathbf{P}\left(A_{1} \cup A_{2} \cup A_{3}\right)=1+1-1=1 \tag{1}
\end{equation*}
$$

Since

$$
\begin{align*}
I_{3} & =\mathbf{P}\left(\left(A_{1} \cup A_{2}\right) \cap A_{3}\right)=\mathbf{P}\left(\left(A_{1} \cap A_{3}\right) \cup\left(A_{2} \cap A_{3}\right)\right) \\
& =\mathbf{P}\left(\left(A_{1} \cap A_{3}\right)\right)+\mathbf{P}\left(\left(A_{2} \cap A_{3}\right)-\mathbf{P}\left(A_{1} \cap A_{2} \cap A_{3}\right)\right.  \tag{2}\\
& =2-\mathbf{P}\left(A_{1} \cap A_{2} \cap A_{3}\right) \tag{3}
\end{align*}
$$

Gathering $\sqrt{1})$ and $(2)$, we get:

$$
\mathbf{P}\left(A_{1} \cap A_{2} \cap A_{3}\right)=2-I_{3}=2-1=1
$$

General case:

Let's use a reasoning by induction on $n$. We assume that for any events $D_{1}, \cdots, D_{n_{0}}$ such that $\mathbf{P}\left(D_{i}\right)=1$, for all $i$ in $\llbracket 1, n_{0} \rrbracket$ then $\mathbf{P}\left(\cap_{i=1}^{n_{0}} D_{i}\right)=1$.

Note that:

$$
\begin{aligned}
1 & =\mathbf{P}\left(A_{1} \cup \cdots \cup A_{n_{0}} \cup A_{n_{0}+1}\right)=\mathbf{P}\left(\left(A_{1} \cup \cdots \cup A_{n_{0}}\right) \cup A_{n_{0}+1}\right) \\
& =\mathbf{P}\left(A_{1} \cup \cdots \cup A_{n_{0}}\right)+\mathbf{P}\left(A_{n_{0}+1}\right)-\mathbf{P}\left(\left(A_{1} \cap A_{n_{0}+1}\right) \cup \cdots \cup\left(A_{n_{0}} \cap A_{n_{0}+1}\right)\right) \\
& =1+1-\mathbf{P}\left(\left(A_{1} \cap A_{n_{0}+1}\right) \cup \cdots \cup\left(A_{n_{0}} \cap A_{n_{0}+1}\right)\right) \\
& =: 1+1-\mathbf{P}\left(B_{1} \cup B_{2} \cup \cdots \cup B_{n_{0}}\right):=2-I_{n_{0}} .
\end{aligned}
$$

where we have set $B_{i}:=A_{i} \cap A_{n_{0}+1}$, for all $i$ in $\llbracket 1, n_{0} \rrbracket$. We hence conclude that $I_{n_{0}}=1$. From the case $n=2$, we immediately deduce that $\mathbf{P}\left(B_{i}\right)=1$, for all $i$ in $\llbracket 1, n_{0} \rrbracket$. We hence are in a situation where $\left(B_{i}\right)_{i \in \llbracket 1, n_{0} \rrbracket}$ is a family of events such that: $\mathbf{P}\left(B_{i}\right)=1$, for all $i$ in $\llbracket 1, n_{0} \rrbracket$. By induction assumption, this entails that:

$$
\mathbf{P}\left(B_{1} \cup B_{2} \cup \cdots \cup B_{n_{0}}\right)=1
$$

Since $\cap_{i=1}^{n_{0}} B_{i}=\cap_{i=1}^{n_{0}+1} A_{i}$, this achieves the proof.

2. The general case is now easy since the sequence of events $\left(D_{N}\right)_{N \in \mathbf{N}^{*}}$, defined by setting:

$$
D_{N}:=\bigcap_{i=1}^{N} A_{i}, \forall N \in \mathbf{N}^{*}
$$

is decreasing. Hence, we have

$$
\mathbf{P}\left(\bigcap_{i=1}^{\infty} A_{i}\right)=\lim _{N \rightarrow \infty} \mathbf{P}\left(\bigcap_{i=1}^{N} A_{i}\right) \stackrel{(Q .1)}{=} \lim _{N \rightarrow \infty} 1=1
$$