We will use the following equality:

$$
\begin{equation*}
\mathbf{P}(A \cup B)=\mathbf{P}(A)+\mathbf{P}(B)-\mathbf{P}(A \cap B) \tag{1}
\end{equation*}
$$

1. In this case, Formula (1) now reads:

$$
\mathbf{P}(A \cup B)=\mathbf{P}(A)+\mathbf{P}(B)=1 / 3+1 / 2=5 / 6
$$

2. If $A$ entails $B$, then $A \subset B$. Thus, Formula (1) now reads:

$$
\mathbf{P}(A \cup B)=\mathbf{P}(A)+\mathbf{P}(B)-\mathbf{P}(A)=\mathbf{P}(B)=1 / 2
$$

3. In this case $\mathbf{P}(A \cap B)=\mathbf{P}(A) \dot{\mathbf{P}}(B)$. Thus, Formula (1) now reads:

$$
\mathbf{P}(A \cup B)=\mathbf{P}(A)+\mathbf{P}(B)-\mathbf{P}(A) \cdot \mathbf{P}(B)=\frac{1}{3}+\frac{1}{2}-\frac{1}{3} \cdot \frac{1}{2}=\frac{5-1}{6}=\frac{2}{3}
$$

4. If $\mathbf{P}(A \mid B)=1 / 2$, then $\mathbf{P}(A \cap B)=\mathbf{P}(B) \cdot \mathbf{P}(A \mid B)=\frac{1}{2} \cdot \frac{1}{2}=\frac{1}{4}$. Thus, Formula (1) now reads:

$$
\mathbf{P}(A \cup B)=\mathbf{P}(A)+\mathbf{P}(B)-\mathbf{P}(A \cap B)=\frac{1}{3}+\frac{1}{2}-\frac{1}{4}=\frac{7}{12}
$$
