Denote $B_{1}$ :"Get 1 and then 2 " and $B_{2}$ :"Get 2 and then 1 ". We easily see that $B=B_{1} \cup B_{2}$. These two latter events being incompatible, we have $\mathbf{P}(B)=\mathbf{P}\left(B_{1}\right)+\mathbf{P}\left(B_{2}\right)$. Moreover, it is clear that the result of the first throw has no impact on the result of the second throw. Therefore $B_{1} \Perp B_{2}$. We hence deduce that:

$$
\begin{aligned}
\mathbf{P}\left(B_{1}\right) & =\mathbf{P}\left(\text { Get } 1 \text { at the } 1^{\text {st }} \text { throw and } 2 \text { at the } 2^{\text {nd }} \text { throw }\right) \\
& =\mathbf{P}\left(\text { Get } 1 \text { at the } 1^{\text {st }} \text { throw }\right) \cdot \mathbf{P}\left(\text { and } 2 \text { at the } 2^{\text {nd }} \text { throw }\right) \\
& =\frac{1}{6} \cdot \frac{1}{6}=\frac{1}{36}
\end{aligned}
$$

In the same manner, one gets $\mathbf{P}\left(B_{2}\right)=\frac{1}{6} \times \frac{1}{6}=\frac{1}{36}$. Finally, and since $B_{1}$ and $B_{2}$ are incompatible, we get:

$$
\mathbf{P}(B)=\mathbf{P}\left(B_{1}\right)+\mathbf{P}\left(B_{2}\right)=\frac{1}{18}
$$

We hence proved that:

$$
\mathbf{P}(B)=\frac{1}{18}
$$
