1. It is clear that the universe $\Omega$ can be defined as $\Omega:=\llbracket 1,6 \rrbracket^{\mathbf{N}^{*}}=\left\{\boldsymbol{u}:=\left(u_{n}\right)_{n \in \mathbf{N}^{*}}, \forall n \in\right.$ $\left.\mathbf{N}^{*}, u_{n} \in \llbracket 1,6 \rrbracket\right\}$.
2. Define $\Lambda:=\bigcap_{k \geqslant 1} A_{k}$ and, for all $n$ in $\mathbf{N}^{*}, \Lambda_{n}:=\bigcap_{k=1}^{n} A_{k}$. It is clear that $\Lambda$ is the event "We get a 6 at every die roll", while $\Lambda_{n}$ is the event "We get a 6 at the first $n^{\text {th }}$ die rolls". Note moreover that we are in a situation of uniform probability. Therefore, one knows that:

$$
\begin{equation*}
\forall k \in \mathbf{N}^{*}, \mathbb{P}\left(A_{k}\right)=\frac{1}{6}=\mathbb{P}\left(A_{1}\right) \tag{1}
\end{equation*}
$$

Moreover, it seems reasonable to assume that $\left(A_{k}\right)_{k \in \mathbf{N}^{*}}$ is a family of independent events, since it is clear that the result of a die roll has no impact on any other die roll.

Besides, using 11) and the independence of the $A_{k}$ 's, one can write, for every $n$ in $\mathbf{N}^{*}$,

$$
\mathbb{P}\left(\Lambda_{n}\right)=\mathbb{P}\left(\bigcap_{k=1}^{n} A_{k}\right) \stackrel{\Perp}{\equiv} \prod_{k=1}^{n} \mathbb{P}\left(A_{k}\right)=\left(\mathbb{P}\left(A_{1}\right)\right)^{n}=\left(\frac{1}{6}\right)^{n}
$$

Moreever, we have $\Lambda \subset \Lambda_{n}$, for every $n \mathbf{N}^{*}$. Thus, one can write:

$$
\begin{equation*}
\forall n \in \mathbf{N}^{*}, 0 \leqslant \mathbb{P}(\Lambda) \leqslant \mathbb{P}\left(\Lambda_{n}\right)=\left(\frac{1}{6}\right)^{n} \tag{2}
\end{equation*}
$$

Taking the limit, when $n$ tends to $\infty$, in the right-hand side of 2D, allows one to claim that $\mathbb{P}(\Lambda)=0$.

3. For all $n$ in $\mathbf{N}^{*}, B_{n}$ is the event "Getting a 6 for the first time, at the $n^{\text {th }}$ die roll". Note moreover that $\cup_{n=1}^{\infty} B_{n}$ is the event "Getting a 6". Besides, one can write $B_{n}=A_{1}^{\mathrm{c}} \cap A_{2}^{\mathrm{c}} \cap$ $\cdots A_{n-1}^{\mathrm{c}} \cap A_{n}$, for every $n$ in $\mathbf{N} \backslash\{0,1\}$, where $A_{k}^{\mathrm{c}}$ denotes the complement event of $A_{k}$. In other words, one has:

$$
\begin{equation*}
\forall n \in \mathbf{N} \backslash\{0,1\}, B_{n}=\left(\bigcap_{k=1}^{n-1} A_{k}^{\mathrm{c}}\right) \cap A_{n} \tag{3}
\end{equation*}
$$

4. Since the $A_{k}$ 's are independent events, the hint given at the end of this exercise allows us to state that, for all $n$ in $\mathbf{N} \backslash\{0,1\},\left(A, A_{k}^{\mathrm{c}}, k \in \llbracket 1, n-1 \rrbracket\right)$ is a family of independent events. Thus, one can write:

$$
\begin{align*}
\forall n \in \mathbf{N} \backslash\{0,1\}, \mathbb{P}\left(B_{n}\right) & =\mathbb{P}\left(\left(\bigcap_{k=1}^{n-1} A_{k}^{\mathrm{c}}\right) \cap A_{n}\right) \stackrel{\Perp}{\Perp}\left(\prod_{k=1}^{n-1} \mathbb{P}\left(A_{k}^{\mathrm{c}}\right)\right) \cdot \mathbb{P}\left(A_{n}\right) \\
& =\left(\mathbb{P}\left(A_{1}^{\mathrm{c}}\right)\right)^{n-1} \cdot \mathbb{P}\left(A_{1}\right)=\left(1-\mathbb{P}\left(A_{1}\right)\right)^{n-1} \cdot \mathbb{P}\left(A_{1}\right) \\
& =\left(\frac{5}{6}\right)^{n-1} \cdot \frac{1}{6} \tag{4}
\end{align*}
$$

Note that $B_{1}=A_{1}, B_{2}=A_{1}^{\mathrm{c}} \cap A_{2}, B_{3}=A_{1}^{\mathrm{c}} \cap A_{2}^{\mathrm{c}} \cap A_{3}$. Moreover, in view of (3), it is clear that the $B_{n}$ are disjoint since, for all $n$ in $\mathbf{N}^{*}, B_{n} \subset A_{n}$ and $B_{n+1} \subset A_{n}^{\mathrm{c}}$. Thus, the Axiom 2 of the definition of a probability allows one to write that $\mathbb{P}\left(\bigcup_{n=1}^{\infty} B_{n}\right)=\sum_{n=1}^{\infty} \mathbb{P}\left(B_{n}\right)$. It is then easy to get, using (4),

$$
\mathbb{P}\left(\bigcup_{n=1}^{\infty} B_{n}\right)=\sum_{n=1}^{\infty} \mathbb{P}\left(B_{n}\right)=\sum_{n=1}^{\infty}\left(\frac{5}{6}\right)^{n-1} \cdot \frac{1}{6}=\frac{1}{6} \sum_{p=0}^{\infty}\left(\frac{5}{6}\right)^{p}=\frac{1}{6} \cdot 1 \cdot\left(\frac{1}{1-\frac{5}{6}}\right)=1
$$

We therefore conclude that the probability to get a six, when rolling a die infinitely many times equals 1.

5. Let us first see what $C_{k}$ means. $C_{1}$ is the event "Not getting a 6 for the first die roll", $C_{2}$ is the event "Not getting a 6 for the first two die rolls". We then have $C_{1}=A_{1}^{\mathrm{c}}$, $C_{2}=A_{1}^{\mathrm{c}} \cap A_{2}^{\mathrm{c}}$. more generally, one can prove that:

$$
\begin{equation*}
\forall n \in \mathbf{N}^{*}, C_{n}=\bigcap_{k=1}^{n} A_{k}^{\mathrm{c}} \tag{5}
\end{equation*}
$$

The independence of the $A_{k}$ 's entails the independence of the $A_{k}^{\mathrm{c}}$ 's. One can thus write:

$\left.\forall n \in \mathbf{N}^{*}, \mathbb{P}\left(C_{n}\right)=\mathbb{P}\left(\bigcap_{k=1}^{n} A_{k}^{\mathrm{c}}\right) \underset{=}{\Perp} \prod_{k=1}^{n} \mathbb{P}\left(A_{k}^{\mathrm{c}}\right)\right)=\prod_{k=1}^{n}\left(1-\mathbb{P}\left(A_{1}^{\mathrm{c}}\right)\right)=\left(1-\mathbb{P}\left(A_{1}^{\mathrm{c}}\right)\right)^{n}=\left(\frac{5}{6}\right)^{n}$.

Finally, in view of the definition of both $B_{\infty}$ and $C_{\infty}$, it is easy to see that $C_{\infty}=B_{\infty}^{\mathrm{c}}$. Thus

$$
\mathbb{P}\left(C_{\infty}\right)=\mathbb{P}\left(B_{\infty}^{\mathrm{c}}\right)=1-\mathbb{P}\left(B_{\infty}\right)=1-1=0
$$

We hence conclude that the probability that we do not get a six, rolling a die infinitely many times, is null.

6. Starting over from (5), one can write:

$$
C_{\infty}=\bigcap_{k=1}^{\infty} A_{k}^{\mathrm{c}}
$$

It would be great to write

$$
\mathbb{P}\left(C_{\infty}\right)=\mathbb{P}\left(\bigcap_{k=1}^{\infty} A_{k}^{\mathrm{c}}\right) \underset{=}{\Perp} \prod_{k=1}^{\infty} \mathbb{P}\left(A_{k}^{\mathrm{c}}\right)
$$

Unfortunately, nothing allows to write the last equality, even if the events of the infinite family $\left(A_{k}^{\mathrm{c}}\right)_{k \in \mathbf{N}^{*}}$ are independent. The problem here lies in the fact that $\left(A_{k}^{\mathrm{c}}\right)_{k \in \mathbf{N}^{*}}$ is not a decreasing $\underbrace{a}$ family of events. However, the family $\left(D_{k}\right)_{k \in \mathbf{N}^{*}}$, defined by setting:

$$
\begin{equation*}
\forall k \in \mathbf{N}^{*}, \quad D_{k}:=\bigcap_{i=1}^{k} A_{i}^{\mathrm{c}} \tag{6}
\end{equation*}
$$

is decreasing since $D_{k+1} \subset D_{k}$, for every $k$ in $\mathbf{N}^{*}$. One can therefore uses the Monotonic limit of events property, one gets:

$$
\begin{aligned}
\mathbb{P}\left(C_{\infty}\right) & =\mathbb{P}\left(\bigcap_{k=1}^{\infty} A_{k}^{\mathrm{c}}\right)=\mathbb{P}\left(\bigcap_{N=1}^{\infty}\left(\bigcap_{k=1}^{N} A_{k}^{\mathrm{c}}\right)\right)=\lim _{N \rightarrow \infty} \mathbb{P}\left(\bigcap_{k=1}^{N} A_{k}^{\mathrm{c}}\right) \underset{N \rightarrow \infty}{\Perp} \lim _{k=1} \prod^{N} \mathbb{P}\left(A_{k}^{\mathrm{c}}\right) \\
& =\lim _{N \rightarrow \infty}\left(\mathbb{P}\left(A_{1}^{\mathrm{c}}\right)\right)^{N}=\lim _{N \rightarrow \infty}\left(1-\mathbb{P}\left(A_{1}\right)\right)^{N}=\lim _{N \rightarrow \infty}\left(\frac{5}{6}\right)^{N}=0
\end{aligned}
$$

We recover the result from the previous question.

${ }^{a}$ for inclusion