
1. By definition, it means that the random variable $X$ can only take to values (that are 1 and $0)$ and that:

$$
\mathbb{P}(X=1)=p \quad \& \quad \mathbb{P}(X=0)=1-p
$$

Since $X$ is a finite random variable, we know that it has a moment of any order and thus that both its expectation and variance exist. Moreover, one has:

$$
\begin{aligned}
& \mathbb{E}[X]=\sum_{k \in X(\Omega)} k \mathbb{P}(X=k)=\sum_{k \in\{0,1\}} k \mathbb{P}(X=k)=\mathbb{P}(X=1)=p \\
& \& \\
& \mathbb{E}\left[X^{2}\right]=\sum_{k \in X(\Omega)} k^{2} \mathbb{P}(X=k)=\sum_{k \in\{0,1\}} k^{2} \mathbb{P}(X=k)=\mathbb{P}(X=1)=p
\end{aligned}
$$

One can therefore write:

$$
\operatorname{Var}(X)=\mathbb{E}\left[X^{2}\right]-(\mathbb{E}[X])^{2}=p-p^{2}=p(1-p)
$$

We hence have proved that:

$$
\mathbb{E}[X]=p \quad \& \quad \operatorname{Var}(X)=p(1-p)
$$

2. By definition, we have:

$$
\forall k \in \llbracket 0, n \rrbracket, \mathbb{P}(X=k)=\binom{n}{k} p^{k}(1-p)^{n-k}
$$

Since $X$ is a finite random variable, we know that it has a moment of any order and thus that both its expectation and variance exist. Moreover, one has:

$$
\begin{aligned}
\mathbb{E}[X] & =\sum_{k=0}^{n}|k| \mathbb{P}(X=k)=\sum_{k=0}^{n} k\binom{n}{k} p^{k}(1-p)^{n-k}=\sum_{k=1}^{n} \frac{k n!}{k!(n-k)!} p^{k} q^{n-k} \\
& =\sum_{k=1}^{n} \frac{n!}{(k-1)!(n-k)!} p^{k} q^{n-k}=n \sum_{k=1}^{n} \frac{(n-1)!}{(k-1)!(n-1-(k-1))!} p^{k} q^{n-k} \\
& =n \sum_{r=0}^{n-1} \frac{(n-1)!}{r!(n-1-r)!} p^{r+1} q^{n-(r+1)}=n p \sum_{r=0}^{n-1}\binom{n-1}{r} p^{r} q^{n-1-r} \\
& =n p(p+q)^{n-1}=n p .
\end{aligned}
$$

By the same manner, one can write:

$$
\begin{aligned}
\mathbb{E}\left[X^{2}\right] & =\sum_{k=0}^{n} k^{2} \mathbb{P}(X=k)=\sum_{k=0}^{n} k^{2}\binom{n}{k} p^{k}(1-p)^{n-k}=\sum_{k=1}^{n} \frac{k^{2} n!}{k!(n-k)!} p^{k} q^{n-k} \\
& =\sum_{k=1}^{n} \frac{k n!}{(k-1)!(n-k)!} p^{k} q^{n-k}=\sum_{k=1}^{n} \frac{((k-1)+1) n!}{(k-1)!(n-k)!} p^{k} q^{n-k} \\
& =\sum_{k=1}^{n} \frac{(k-1) n!}{(k-1)!(n-k)!} p^{k} q^{n-k}+\sum_{k=1}^{n} \frac{n!}{(k-1)!(n-k)!} p^{k} q^{n-k} \\
& =\sum_{k=2}^{n} \frac{(k-1) n!}{(k-1)!(n-k)!} p^{k} q^{n-k}+\mathbb{E}[X]=\sum_{k=2}^{n} \frac{n!}{(k-2)!(n-k)!} p^{k} q^{n-k}+n p \\
& =n(n-1) p^{2} \sum_{k=2}^{n} \frac{(n-2)!}{(k-2)!(n-2-(k-2))!} p^{k-2} q^{n-2-(k-2)}+n p \\
& =n(n-1) p^{2} \sum_{r=0}^{n-2} \frac{(n-2)!}{r!(n-2-r)!} p^{r} q^{n-2-r}+n p \\
& =n(n-1) p^{2} \sum_{r=0}^{n-2}\binom{n-2}{r} p^{r} q^{n-2-r}+n p=n(n-1) p^{2}(p+q)^{n-2}+n p \\
& =n(n-1) p^{2}+n p
\end{aligned}
$$

It is therefore easy to conclude that:

$$
\begin{aligned}
\operatorname{Var}(X) & =\mathbb{E}\left[X^{2}\right]-(\mathbb{E}[X])^{2}=n(n-1) p^{2}+n p-(n p)^{2}=n p((n-1) p+1-n p) \\
& =n p(1-p)
\end{aligned}
$$

We hence have proved that:

$$
\mathbb{E}[X]=n p \quad \& \quad \operatorname{Var}(X)=n p(1-p)
$$

3. By definition, it means that the random variable $X$ can only take the $x_{i}$ as values. Moreover, we have:

$$
\forall i \in \llbracket 1, n \rrbracket, \mathbb{P}\left(X=x_{i}\right)=\frac{1}{n}
$$

Since $X$ is a finite random variable, we know that it has a moment of any order and thus that both its expectation and variance exist. Moreover, one has:

$$
\mathbb{E}[X]=\sum_{\alpha \in X(\Omega)} \alpha \mathbb{P}(X=\alpha)=\sum_{k=1}^{n} x_{k} \mathbb{P}\left(X=x_{k}\right)=\sum_{k=1}^{n} x_{k} \frac{1}{n}=\frac{\sum_{k=1}^{n} x_{k}}{n}
$$

$\&$

$$
\mathbb{E}\left[X^{2}\right]=\sum_{\alpha \in X(\Omega)} \alpha^{2} \mathbb{P}(X=\alpha)=\sum_{k=1}^{n} x_{k}^{2} \mathbb{P}\left(X=x_{k}\right)=\sum_{k=1}^{n} x_{k}^{2} \frac{1}{n}=\frac{\sum_{k=1}^{n} x_{k}^{2}}{n}
$$

One can therefore write:

$$
\operatorname{Var}(X)=\mathbb{E}\left[X^{2}\right]-(\mathbb{E}[X])^{2}=\frac{\sum_{k=1}^{n} x_{k}^{2}}{n}-\left(\frac{\sum_{k=1}^{n} x_{k}}{n}\right)^{2}
$$

We hence have proved that:

$$
\mathbb{E}[X]=\frac{\sum_{k=1}^{n} x_{k}^{2}}{n} \quad \& \quad \operatorname{Var}(X)=\frac{\sum_{k=1}^{n} x_{k}^{2}}{n}-\left(\frac{\sum_{k=1}^{n} x_{k}}{n}\right)^{2}
$$